bin/utils.ml
@@ -1,6 +1,7 @@
 
 open Elykseer__Lxr
-open Elykseer__Lxr.Backup
+open Elykseer__Lxr.Block
+open Elykseer__Lxr.Environment
 open Elykseer__Lxr.Filetypes
 
 let fi2s fi = "Fileinformation: fname = \"" ^ fi.fname ^ "\""
@@ -12,11 +13,15 @@ let fi2s fi = "Fileinformation: fname = \"" ^ fi.fname ^ "\""
 
 let b2s b = "Block: blockid = " ^ (string_of_int @@ Conversion.p2i @@ b.blockid)
           ^ ", blocksize = " ^ (string_of_int @@ Conversion.n2i @@ b.blocksize)
+          ^ ", filepos = " ^ (string_of_int @@ Conversion.n2i @@ b.filepos)
           ^ ", blockaid = " ^ (string_of_int @@ Conversion.p2i @@ b.blockaid)
+          ^ ", blockapos = " ^ (string_of_int @@ Conversion.n2i @@ b.blockapos)
+
+let fibs2s fibs = "\n  " ^ fi2s (bfi fibs)
+          ^ "\n                 , blocks = " ^ (string_of_int @@ List.length @@ blocks fibs) ^ "@[" ^ (String.concat "; " (map b2s (blocks fibs))) ^ "]"
 
 let e2s e = "Environment: cur_assembly = " ^ (string_of_int @@ Conversion.p2i @@ Assembly.aid @@ cur_assembly e)
           ^ ", count_input_bytes = " ^ (string_of_int @@ Conversion.n2i @@ count_input_bytes e)
-          ^ ", files = " ^ (string_of_int @@ List.length @@ files e) ^ "@[" ^ (String.concat "; " (map fi2s (files e))) ^ "]"
-          ^ ", blocks = " ^ (string_of_int @@ List.length @@ blocks e) ^ "@[" ^ (String.concat "; " (map b2s (blocks e))) ^ "]"
+          ^ ", files = " ^ (string_of_int @@ List.length @@ files e) ^ "@[" ^ (String.concat "; " (map fibs2s (files e))) ^ "]"
           ^ "\n."
 
