theories/Block.v
@@ -1,0 +1,31 @@
+(**
+      e L y K s e e R
+*)
+
+Module Export Block.
+
+Require Import NArith.
+From Coq Require Import NArith.BinNat.
+(* From Coq Require Import Strings.String Strings.Byte. *)
+
+Open Scope N_scope.
+
+From LXR Require Import Filetypes.
+
+(* Definition block := list byte. *)
+Record blockinformation : Type :=
+    mkblockinformation
+        { blockid : positive
+        ; blocksize : N
+        ; filepos : N
+        ; blockaid : positive
+        ; blockapos : N
+        }.
+
+Record fileblocks : Type :=
+    mkfileblocks
+        { bfi : fileinformation
+        ; blocks : list blockinformation
+        }.
+
+End Block.
