theories/Configuration.v
@@ -1,0 +1,17 @@
+(**
+      e L y K s e e R
+*)
+
+Module Export Configuration.
+
+Require Import PArith.
+From Coq Require Import Strings.String.
+
+Record configuration : Type :=
+    mkconfiguration
+        { num_chunks : positive
+        ; path_chunks : string
+        ; path_meta : string
+        }.
+
+End Configuration.
