theories/Environment.v
@@ -1,0 +1,38 @@
+(**
+      e L y K s e e R
+*)
+
+Module Export Environment.
+
+Require Import NArith.
+From Coq Require Import NArith.BinNat.
+Open Scope N_scope.
+
+From LXR Require Import Assembly.
+From LXR Require Import Block.
+From LXR Require Import Configuration.
+From LXR Require Import Filetypes.
+
+Record environment : Type :=
+    mkenvironment
+        { cur_assembly : assembly
+        ; count_input_bytes : N
+        ; files : list fileblocks
+        }.
+Definition initial_environment (c : configuration) : environment :=
+    {| cur_assembly := first_assembly (num_chunks c)
+    ;  count_input_bytes := 0%N
+    ;  files := nil
+    |}.
+Definition env_set_assembly (e : environment) (a : assembly) : environment :=
+    {| cur_assembly := a
+    ;  count_input_bytes := count_input_bytes e
+    ;  files := files e
+    |}.
+Definition env_add_file (e : environment) (fibs : fileblocks) : environment :=
+    {| cur_assembly := cur_assembly e
+    ; count_input_bytes := count_input_bytes e + fsize (bfi fibs)
+    ; files := fibs :: files e
+    |}.
+
+End Environment.
