theories/Example.v
@@ -13,6 +13,9 @@ Open Scope positive_scope.
 Open Scope N_scope.
 
 From LXR Require Import Backup.
+From LXR Require Import Block.
+From LXR Require Import Configuration.
+From LXR Require Import Environment.
 From LXR Require Import Filesupport.
 From LXR Require Import Filetypes.
 
@@ -31,17 +34,36 @@ Require Import LXR.Assembly.
 Example env0 (c : configuration) : environment :=
     initial_environment c.
 
+Example fi_t1_dat : fileinformation := {| fname := "t1.dat"; fsize := 33; fowner := "me"; fpermissions := 644; fmodified := ""; fchecksum := "" |}.
+
 Lemma test1 : 
     let e := env0 config0 in
-    let fi := {| fname := "t1.dat"; fsize := 33; fowner := "me"; fpermissions := 644; fmodified := ""; fchecksum := "" |} in
-    let bi := {| blockid := 1; blocksize := 33; blockaid := 1 |} in
+    let fi := fi_t1_dat in
+    let bi := {| blockid := 1; blocksize := 33; filepos := 0; blockaid := 1; blockapos := 0 |} in
     backup_file config0 e "t1.dat" =
-    {| cur_assembly := first_assembly (num_chunks config0) 
+    {| cur_assembly := {|
+                        nchunks := 16;
+                        aid := 1;
+                        valid := valid_assembly_size 16;
+                        apos := 33; (*N.min (assemblysz config0) 33;*)
+                        encrypted := false;
+                        chunks := mk_chunk_list 16 1
+                       |} 
     ;  count_input_bytes := 33
-    ;  files := fi :: nil
-    ;  blocks := bi :: nil
+    ;  files := {| bfi:= fi; blocks := bi :: nil |} :: nil
     |}.
-Proof. Admitted.
+Proof. intros.
+    unfold backup_file.
+    replace (get_file_information "t1.dat") with fi.
+    simpl.
+    vm_compute (N.min (assemblysz config0) 33).
+    
+    unfold add_data.
+    unfold env_set_assembly.
+    unfold env_add_file. simpl.
+
+    reflexivity.
+ Admitted. (* the remaining: fi = get_file_information "t1.dat" *)
 
 
 End Example.
